cfrontend/Cexec.v
@@ -25,6 +25,8 @@ Require Import Memory.
 Require Import Events.
 Require Import Globalenvs.
 Require Import Determinism.
+Require Import Ctypes.
+Require Import Cop.
 Require Import Csyntax.
 Require Import Csem.
 Require Cstrategy.
