cfrontend/Cop.v
@@ -1,0 +1,822 @@
+(* *********************************************************************)
+(*                                                                     *)
+(*              The Compcert verified compiler                         *)
+(*                                                                     *)
+(*          Xavier Leroy, INRIA Paris-Rocquencourt                     *)
+(*                                                                     *)
+(*  Copyright Institut National de Recherche en Informatique et en     *)
+(*  Automatique.  All rights reserved.  This file is distributed       *)
+(*  under the terms of the GNU General Public License as published by  *)
+(*  the Free Software Foundation, either version 2 of the License, or  *)
+(*  (at your option) any later version.  This file is also distributed *)
+(*  under the terms of the INRIA Non-Commercial License Agreement.     *)
+(*                                                                     *)
+(* *********************************************************************)
+
+(** Arithmetic and logical operators for the Compcert C and Clight languages *)
+
+Require Import Coqlib.
+Require Import AST.
+Require Import Integers.
+Require Import Floats.
+Require Import Values.
+Require Import Memory.
+Require Import Ctypes.
+
+(** * Syntax of operators. *)
+
+Inductive unary_operation : Type :=
+  | Onotbool : unary_operation          (**r boolean negation ([!] in C) *)
+  | Onotint : unary_operation           (**r integer complement ([~] in C) *)
+  | Oneg : unary_operation.             (**r opposite (unary [-]) *)
+
+Inductive binary_operation : Type :=
+  | Oadd : binary_operation             (**r addition (binary [+]) *)
+  | Osub : binary_operation             (**r subtraction (binary [-]) *)
+  | Omul : binary_operation             (**r multiplication (binary [*]) *)
+  | Odiv : binary_operation             (**r division ([/]) *)
+  | Omod : binary_operation             (**r remainder ([%]) *)
+  | Oand : binary_operation             (**r bitwise and ([&]) *)
+  | Oor : binary_operation              (**r bitwise or ([|]) *)
+  | Oxor : binary_operation             (**r bitwise xor ([^]) *)
+  | Oshl : binary_operation             (**r left shift ([<<]) *)
+  | Oshr : binary_operation             (**r right shift ([>>]) *)
+  | Oeq: binary_operation               (**r comparison ([==]) *)
+  | One: binary_operation               (**r comparison ([!=]) *)
+  | Olt: binary_operation               (**r comparison ([<]) *)
+  | Ogt: binary_operation               (**r comparison ([>]) *)
+  | Ole: binary_operation               (**r comparison ([<=]) *)
+  | Oge: binary_operation.              (**r comparison ([>=]) *)
+
+Inductive incr_or_decr : Type := Incr | Decr.
+
+(** * Type classification and semantics of operators. *)
+
+(** Most C operators are overloaded (they apply to arguments of various
+  types) and their semantics depend on the types of their arguments.
+  The following [classify_*] functions take as arguments the types
+  of the arguments of an operation.  They return enough information
+  to resolve overloading for this operator applications, such as
+  ``both arguments are floats'', or ``the first is a pointer
+  and the second is an integer''.  This classification is used in the
+  compiler (module [Cshmgen]) to resolve overloading statically.
+
+  The [sem_*] functions below compute the result of an operator
+  application.  Since operators are overloaded, the result depends
+  both on the static types of the arguments and on their run-time values.
+  The corresponding [classify_*] function is first called on the 
+  types of the arguments to resolve static overloading.  It is then
+  followed by a case analysis on the values of the arguments. *)
+
+(** ** Casts and truth values *)
+
+Inductive classify_cast_cases : Type :=
+  | cast_case_neutral                   (**r int|pointer -> int32|pointer *)
+  | cast_case_i2i (sz2:intsize) (si2:signedness)   (**r int -> int *)
+  | cast_case_f2f (sz2:floatsize)                  (**r float -> float *)
+  | cast_case_i2f (si1:signedness) (sz2:floatsize) (**r int -> float *)
+  | cast_case_f2i (sz2:intsize) (si2:signedness)   (**r float -> int *)
+  | cast_case_f2bool                    (**r float -> bool *)
+  | cast_case_p2bool                    (**r pointer -> bool *)
+  | cast_case_struct (id1: ident) (fld1: fieldlist) (id2: ident) (fld2: fieldlist) (**r struct -> struct *)
+  | cast_case_union (id1: ident) (fld1: fieldlist) (id2: ident) (fld2: fieldlist) (**r union -> union *)
+  | cast_case_void                                 (**r any -> void *)
+  | cast_case_default.
+
+Function classify_cast (tfrom tto: type) : classify_cast_cases :=
+  match tto, tfrom with
+  | Tint I32 si2 _, (Tint _ _ _ | Tpointer _ _ | Tarray _ _ _ | Tfunction _ _) => cast_case_neutral
+  | Tint IBool _ _, Tfloat _ _ => cast_case_f2bool
+  | Tint IBool _ _, (Tpointer _ _ | Tarray _ _ _ | Tfunction _ _) => cast_case_p2bool
+  | Tint sz2 si2 _, Tint sz1 si1 _ => cast_case_i2i sz2 si2
+  | Tint sz2 si2 _, Tfloat sz1 _ => cast_case_f2i sz2 si2
+  | Tfloat sz2 _, Tfloat sz1 _ => cast_case_f2f sz2
+  | Tfloat sz2 _, Tint sz1 si1 _ => cast_case_i2f si1 sz2
+  | Tpointer _ _, (Tint _ _ _ | Tpointer _ _ | Tarray _ _ _ | Tfunction _ _) => cast_case_neutral
+  | Tstruct id2 fld2 _, Tstruct id1 fld1 _ => cast_case_struct id1 fld1 id2 fld2
+  | Tunion id2 fld2 _, Tunion id1 fld1 _ => cast_case_union id1 fld1 id2 fld2
+  | Tvoid, _ => cast_case_void
+  | _, _ => cast_case_default
+  end.
+
+(** Semantics of casts.  [sem_cast v1 t1 t2 = Some v2] if value [v1],
+  viewed with static type [t1], can be cast to type [t2],
+  resulting in value [v2].  *)
+
+Definition cast_int_int (sz: intsize) (sg: signedness) (i: int) : int :=
+  match sz, sg with
+  | I8, Signed => Int.sign_ext 8 i
+  | I8, Unsigned => Int.zero_ext 8 i
+  | I16, Signed => Int.sign_ext 16 i
+  | I16, Unsigned => Int.zero_ext 16 i 
+  | I32, _ => i
+  | IBool, _ => if Int.eq i Int.zero then Int.zero else Int.one
+  end.
+
+Definition cast_int_float (si : signedness) (i: int) : float :=
+  match si with
+  | Signed => Float.floatofint i
+  | Unsigned => Float.floatofintu i
+  end.
+
+Definition cast_float_int (si : signedness) (f: float) : option int :=
+  match si with
+  | Signed => Float.intoffloat f
+  | Unsigned => Float.intuoffloat f
+  end.
+
+Definition cast_float_float (sz: floatsize) (f: float) : float :=
+  match sz with
+  | F32 => Float.singleoffloat f
+  | F64 => f
+  end.
+
+Function sem_cast (v: val) (t1 t2: type) : option val :=
+  match classify_cast t1 t2 with
+  | cast_case_neutral =>
+      match v with
+      | Vint _ | Vptr _ _ => Some v
+      | _ => None
+      end
+  | cast_case_i2i sz2 si2 =>
+      match v with
+      | Vint i => Some (Vint (cast_int_int sz2 si2 i))
+      | _ => None
+      end
+  | cast_case_f2f sz2 =>
+      match v with
+      | Vfloat f => Some (Vfloat (cast_float_float sz2 f))
+      | _ => None
+      end
+  | cast_case_i2f si1 sz2 =>
+      match v with
+      | Vint i => Some (Vfloat (cast_float_float sz2 (cast_int_float si1 i)))
+      | _ => None
+      end
+  | cast_case_f2i sz2 si2 =>
+      match v with
+      | Vfloat f =>
+          match cast_float_int si2 f with
+          | Some i => Some (Vint (cast_int_int sz2 si2 i))
+          | None => None
+          end
+      | _ => None
+      end
+  | cast_case_f2bool =>
+      match v with
+      | Vfloat f =>
+          Some(Vint(if Float.cmp Ceq f Float.zero then Int.zero else Int.one))
+      | _ => None
+      end
+  | cast_case_p2bool =>
+      match v with
+      | Vint i => Some (Vint (cast_int_int IBool Signed i))
+      | Vptr _ _ => Some (Vint Int.one)
+      | _ => None
+      end
+  | cast_case_struct id1 fld1 id2 fld2 =>
+      if ident_eq id1 id2 && fieldlist_eq fld1 fld2 then Some v else None
+  | cast_case_union id1 fld1 id2 fld2 =>
+      if ident_eq id1 id2 && fieldlist_eq fld1 fld2 then Some v else None
+  | cast_case_void =>
+      Some v
+  | cast_case_default =>
+      None
+  end.
+
+(** The following describes types that can be interpreted as a boolean:
+  integers, floats, pointers.  It is used for the semantics of 
+  the [!] and [?] operators, as well as the [if], [while], [for] statements. *)
+
+Inductive classify_bool_cases : Type :=
+  | bool_case_i                           (**r integer *)
+  | bool_case_f                           (**r float *)
+  | bool_case_p                           (**r pointer *)
+  | bool_default.
+
+Definition classify_bool (ty: type) : classify_bool_cases :=
+  match typeconv ty with
+  | Tint _ _ _ => bool_case_i
+  | Tpointer _ _ => bool_case_p
+  | Tfloat _ _ => bool_case_f
+  | _ => bool_default
+  end.
+
+(** Interpretation of values as truth values.
+  Non-zero integers, non-zero floats and non-null pointers are
+  considered as true.  The integer zero (which also represents
+  the null pointer) and the float 0.0 are false. *)
+
+Function bool_val (v: val) (t: type) : option bool :=
+  match classify_bool t with
+  | bool_case_i =>
+      match v with
+      | Vint n => Some (negb (Int.eq n Int.zero))
+      | _ => None
+      end
+  | bool_case_f =>
+      match v with
+      | Vfloat f => Some (negb (Float.cmp Ceq f Float.zero))
+      | _ => None
+      end
+  | bool_case_p =>
+      match v with
+      | Vint n => Some (negb (Int.eq n Int.zero))
+      | Vptr b ofs => Some true
+      | _ => None
+      end
+  | bool_default => None
+  end.
+
+(** Common-sense relation between Boolean value and casting to [_Bool] type. *)
+
+Lemma cast_bool_bool_val:
+  forall v t,
+  sem_cast v t (Tint IBool Signed noattr) =
+  match bool_val v t with None => None | Some b => Some(Val.of_bool b) end.
+Proof.
+  intros.
+  assert (A: classify_bool t =
+    match t with
+    | Tint _ _ _ => bool_case_i
+    | Tpointer _ _ | Tarray _ _ _ | Tfunction _ _ => bool_case_p
+    | Tfloat _ _ => bool_case_f
+    | _ => bool_default
+    end).
+  unfold classify_bool; destruct t; simpl; auto. destruct i; auto. destruct s; auto.
+
+  unfold bool_val. rewrite A. unfold sem_cast. destruct t; simpl; auto; destruct v; auto.
+  destruct (Int.eq i0 Int.zero); auto. 
+  destruct (Float.cmp Ceq f0 Float.zero); auto.
+  destruct (Int.eq i Int.zero); auto. 
+  destruct (Int.eq i Int.zero); auto. 
+  destruct (Int.eq i Int.zero); auto. 
+Qed.
+
+(** ** Unary operators *)
+
+(** *** Boolean negation *)
+
+Function sem_notbool (v: val) (ty: type) : option val :=
+  match classify_bool ty with
+  | bool_case_i =>
+      match v with
+      | Vint n => Some (Val.of_bool (Int.eq n Int.zero))
+      | _ => None
+      end
+  | bool_case_f =>
+      match v with
+      | Vfloat f => Some (Val.of_bool (Float.cmp Ceq f Float.zero))
+      | _ => None
+      end
+  | bool_case_p =>
+      match v with
+      | Vint n => Some (Val.of_bool (Int.eq n Int.zero))
+      | Vptr _ _ => Some Vfalse
+      | _ => None
+      end
+  | bool_default => None
+  end.
+
+(** Common-sense relation between Boolean value and Boolean negation. *)
+
+Lemma notbool_bool_val:
+  forall v t,
+  sem_notbool v t =
+  match bool_val v t with None => None | Some b => Some(Val.of_bool (negb b)) end.
+Proof.
+  intros. unfold sem_notbool, bool_val. 
+  destruct (classify_bool t); auto; destruct v; auto; rewrite negb_involutive; auto.
+Qed.
+
+(** *** Opposite *)
+
+Inductive classify_neg_cases : Type :=
+  | neg_case_i(s: signedness)              (**r int *)
+  | neg_case_f                             (**r float *)
+  | neg_default.
+
+Definition classify_neg (ty: type) : classify_neg_cases :=
+  match ty with
+  | Tint I32 Unsigned _ => neg_case_i Unsigned
+  | Tint _ _ _ => neg_case_i Signed
+  | Tfloat _ _ => neg_case_f
+  | _ => neg_default
+  end.
+
+Function sem_neg (v: val) (ty: type) : option val :=
+  match classify_neg ty with
+  | neg_case_i sg =>
+      match v with
+      | Vint n => Some (Vint (Int.neg n))
+      | _ => None
+      end
+  | neg_case_f =>
+      match v with
+      | Vfloat f => Some (Vfloat (Float.neg f))
+      | _ => None
+      end
+  | neg_default => None
+  end.
+
+(** *** Bitwise complement *)
+
+Inductive classify_notint_cases : Type :=
+  | notint_case_i(s: signedness)              (**r int *)
+  | notint_default.
+
+Definition classify_notint (ty: type) : classify_notint_cases :=
+  match ty with
+  | Tint I32 Unsigned _ => notint_case_i Unsigned
+  | Tint _ _ _ => notint_case_i Signed
+  | _ => notint_default
+  end.
+
+Function sem_notint (v: val) (ty: type): option val :=
+  match classify_notint ty with
+  | notint_case_i sg =>
+      match v with
+      | Vint n => Some (Vint (Int.xor n Int.mone))
+      | _ => None
+      end
+  | notint_default => None
+  end.
+
+(** ** Binary operators *)
+
+(** For binary operations, the "usual binary conversions", adapted to a 32-bit
+  platform, state that:
+- If both arguments are of integer type, an integer operation is performed.
+  For operations that behave differently at unsigned and signed types
+  (e.g. division, modulus, comparisons), the unsigned operation is selected
+  if at least one of the arguments is of type "unsigned int32", otherwise
+  the signed operation is performed.
+- If both arguments are of float type, a float operation is performed.
+  We choose to perform all float arithmetic in double precision,
+  even if both arguments are single-precision floats.
+- If one argument has integer type and the other has float type,
+  we convert the integer argument to float, then perform the float operation.
+*)
+
+(** *** Addition *)
+
+Inductive classify_add_cases : Type :=
+  | add_case_ii(s: signedness)         (**r int, int *)
+  | add_case_ff                        (**r float, float *)
+  | add_case_if(s: signedness)         (**r int, float *)
+  | add_case_fi(s: signedness)         (**r float, int *)
+  | add_case_pi(ty: type)(a: attr)     (**r pointer, int *)
+  | add_case_ip(ty: type)(a: attr)     (**r int, pointer *)
+  | add_default.
+
+Definition classify_add (ty1: type) (ty2: type) :=
+  match typeconv ty1, typeconv ty2 with
+  | Tint I32 Unsigned _, Tint _ _ _ => add_case_ii Unsigned
+  | Tint _ _ _, Tint I32 Unsigned _ => add_case_ii Unsigned
+  | Tint _ _ _, Tint _ _ _ => add_case_ii Signed
+  | Tfloat _ _, Tfloat _ _ => add_case_ff
+  | Tint _ sg _, Tfloat _ _ => add_case_if sg
+  | Tfloat _ _, Tint _ sg _ => add_case_fi sg
+  | Tpointer ty a, Tint _ _ _ => add_case_pi ty a
+  | Tint _ _ _, Tpointer ty a => add_case_ip ty a
+  | _, _ => add_default
+  end.
+
+Function sem_add (v1:val) (t1:type) (v2: val) (t2:type) : option val :=
+  match classify_add t1 t2 with 
+  | add_case_ii sg =>                   (**r integer addition *)
+      match v1, v2 with
+      | Vint n1, Vint n2 => Some (Vint (Int.add n1 n2))
+      | _,  _ => None
+      end
+  | add_case_ff =>                      (**r float addition *)
+      match v1, v2 with
+      | Vfloat n1, Vfloat n2 => Some (Vfloat (Float.add n1 n2))
+      | _,  _ => None
+      end
+  | add_case_if sg =>                   (**r int plus float *)
+      match v1, v2 with
+      | Vint n1, Vfloat n2 => Some (Vfloat (Float.add (cast_int_float sg n1) n2))
+      | _, _ => None
+      end
+  | add_case_fi sg =>                   (**r float plus int *)
+      match v1, v2 with
+      | Vfloat n1, Vint n2 => Some (Vfloat (Float.add n1 (cast_int_float sg n2)))
+      | _, _ => None
+      end
+  | add_case_pi ty _ =>                 (**r pointer plus integer *)
+      match v1,v2 with
+      | Vptr b1 ofs1, Vint n2 => 
+        Some (Vptr b1 (Int.add ofs1 (Int.mul (Int.repr (sizeof ty)) n2)))
+      | _,  _ => None
+      end   
+  | add_case_ip ty _ =>                 (**r integer plus pointer *)
+      match v1,v2 with
+      | Vint n1, Vptr b2 ofs2 => 
+        Some (Vptr b2 (Int.add ofs2 (Int.mul (Int.repr (sizeof ty)) n1)))
+      | _,  _ => None
+      end   
+  | add_default => None
+end.
+
+(** *** Subtraction *)
+
+Inductive classify_sub_cases : Type :=
+  | sub_case_ii(s: signedness)          (**r int , int *)
+  | sub_case_ff                         (**r float , float *)
+  | sub_case_if(s: signedness)          (**r int, float *)
+  | sub_case_fi(s: signedness)          (**r float, int *)
+  | sub_case_pi(ty: type)               (**r pointer, int *)
+  | sub_case_pp(ty: type)               (**r pointer, pointer *)
+  | sub_default.
+
+Definition classify_sub (ty1: type) (ty2: type) :=
+  match typeconv ty1, typeconv ty2 with
+  | Tint I32 Unsigned _, Tint _ _ _ => sub_case_ii Unsigned
+  | Tint _ _ _, Tint I32 Unsigned _ => sub_case_ii Unsigned
+  | Tint _ _ _, Tint _ _ _ => sub_case_ii Signed
+  | Tfloat _ _ , Tfloat _ _ => sub_case_ff
+  | Tint _ sg _, Tfloat _ _ => sub_case_if sg
+  | Tfloat _ _, Tint _ sg _ => sub_case_fi sg
+  | Tpointer ty _, Tint _ _ _ => sub_case_pi ty
+  | Tpointer ty _ , Tpointer _ _ => sub_case_pp ty
+  | _ ,_ => sub_default
+  end.
+
+Function sem_sub (v1:val) (t1:type) (v2: val) (t2:type) : option val :=
+  match classify_sub t1 t2 with
+  | sub_case_ii sg =>            (**r integer subtraction *)
+      match v1,v2 with
+      | Vint n1, Vint n2 => Some (Vint (Int.sub n1 n2))
+      | _,  _ => None
+      end 
+  | sub_case_ff =>               (**r float subtraction *)
+      match v1,v2 with
+      | Vfloat f1, Vfloat f2 => Some (Vfloat(Float.sub f1 f2))
+      | _,  _ => None
+      end
+  | sub_case_if sg =>            (**r int minus float *)
+      match v1, v2 with
+      | Vint n1, Vfloat n2 => Some (Vfloat (Float.sub (cast_int_float sg n1) n2))
+      | _, _ => None
+      end
+  | sub_case_fi sg =>            (**r float minus int *)
+      match v1, v2 with
+      | Vfloat n1, Vint n2 => Some (Vfloat (Float.sub n1 (cast_int_float sg n2)))
+      | _, _ => None
+      end
+  | sub_case_pi ty =>            (**r pointer minus integer *)
+      match v1,v2 with
+      | Vptr b1 ofs1, Vint n2 => 
+            Some (Vptr b1 (Int.sub ofs1 (Int.mul (Int.repr (sizeof ty)) n2)))
+      | _,  _ => None
+      end
+  | sub_case_pp ty =>          (**r pointer minus pointer *)
+      match v1,v2 with
+      | Vptr b1 ofs1, Vptr b2 ofs2 =>
+          if zeq b1 b2 then
+            if Int.eq (Int.repr (sizeof ty)) Int.zero then None
+            else Some (Vint (Int.divu (Int.sub ofs1 ofs2) (Int.repr (sizeof ty))))
+          else None
+      | _, _ => None
+      end
+  | sub_default => None
+  end.
+ 
+(** *** Multiplication *)
+
+Inductive classify_mul_cases : Type:=
+  | mul_case_ii(s: signedness) (**r int , int *)
+  | mul_case_ff                (**r float , float *)
+  | mul_case_if(s: signedness) (**r int, float *)
+  | mul_case_fi(s: signedness) (**r float, int *)
+  | mul_default.
+
+Definition classify_mul (ty1: type) (ty2: type) :=
+  match typeconv ty1, typeconv ty2 with
+  | Tint I32 Unsigned _, Tint _ _ _ => mul_case_ii Unsigned
+  | Tint _ _ _, Tint I32 Unsigned _ => mul_case_ii Unsigned
+  | Tint _ _ _, Tint _ _ _ => mul_case_ii Signed
+  | Tfloat _ _ , Tfloat _ _ => mul_case_ff
+  | Tint _ sg _, Tfloat _ _ => mul_case_if sg
+  | Tfloat _ _, Tint _ sg _ => mul_case_fi sg
+  | _,_  => mul_default
+end.
+
+Function sem_mul (v1:val) (t1:type) (v2: val) (t2:type) : option val :=
+ match classify_mul t1 t2 with
+  | mul_case_ii sg =>
+      match v1,v2 with
+      | Vint n1, Vint n2 => Some (Vint (Int.mul n1 n2))
+      | _,  _ => None
+      end
+  | mul_case_ff =>
+      match v1,v2 with
+      | Vfloat f1, Vfloat f2 => Some (Vfloat (Float.mul f1 f2))
+      | _,  _ => None
+      end
+  | mul_case_if sg =>
+      match v1, v2 with
+      | Vint n1, Vfloat n2 => Some (Vfloat (Float.mul (cast_int_float sg n1) n2))
+      | _, _ => None
+      end
+  | mul_case_fi sg =>
+      match v1, v2 with
+      | Vfloat n1, Vint n2 => Some (Vfloat (Float.mul n1 (cast_int_float sg n2)))
+      | _, _ => None
+      end
+  | mul_default =>
+      None
+end.
+
+(** *** Division *)
+
+Inductive classify_div_cases : Type:=
+  | div_case_ii(s: signedness) (**r int , int *)
+  | div_case_ff                (**r float , float *)
+  | div_case_if(s: signedness) (**r int, float *)
+  | div_case_fi(s: signedness) (**r float, int *)
+  | div_default.
+
+Definition classify_div (ty1: type) (ty2: type) :=
+  match typeconv ty1, typeconv ty2 with
+  | Tint I32 Unsigned _, Tint _ _ _ => div_case_ii Unsigned
+  | Tint _ _ _, Tint I32 Unsigned _ => div_case_ii Unsigned
+  | Tint _ _ _, Tint _ _ _ => div_case_ii Signed
+  | Tfloat _ _ , Tfloat _ _ => div_case_ff
+  | Tint _ sg _, Tfloat _ _ => div_case_if sg
+  | Tfloat _ _, Tint _ sg _ => div_case_fi sg
+  | _,_  => div_default
+end.
+
+Function sem_div (v1:val) (t1:type) (v2: val) (t2:type) : option val :=
+   match classify_div t1 t2 with
+  | div_case_ii Unsigned =>
+      match v1,v2 with
+      | Vint n1, Vint n2 =>
+          if Int.eq n2 Int.zero then None else Some (Vint (Int.divu n1 n2))
+      | _,_ => None
+      end
+  | div_case_ii Signed =>
+      match v1,v2 with
+       | Vint n1, Vint n2 =>
+          if Int.eq n2 Int.zero
+          || Int.eq n1 (Int.repr Int.min_signed) && Int.eq n2 Int.mone
+          then None else Some (Vint(Int.divs n1 n2))
+      | _,_ => None
+      end
+  | div_case_ff =>
+      match v1,v2 with
+      | Vfloat f1, Vfloat f2 => Some (Vfloat(Float.div f1 f2))
+      | _,  _ => None
+      end 
+  | div_case_if sg =>
+      match v1, v2 with
+      | Vint n1, Vfloat n2 => Some (Vfloat (Float.div (cast_int_float sg n1) n2))
+      | _, _ => None
+      end
+  | div_case_fi sg =>
+      match v1, v2 with
+      | Vfloat n1, Vint n2 => Some (Vfloat (Float.div n1 (cast_int_float sg n2)))
+      | _, _ => None
+      end
+  | div_default =>
+      None
+end.
+
+(** *** Integer-only binary operations: modulus, bitwise "and", "or", and "xor" *)
+
+Inductive classify_binint_cases : Type:=
+  | binint_case_ii(s: signedness) (**r int , int *)
+  | binint_default.
+
+Definition classify_binint (ty1: type) (ty2: type) :=
+  match typeconv ty1, typeconv ty2 with
+  | Tint I32 Unsigned _, Tint _ _ _ => binint_case_ii Unsigned
+  | Tint _ _ _, Tint I32 Unsigned _ => binint_case_ii Unsigned
+  | Tint _ _ _, Tint _ _ _ => binint_case_ii Signed
+  | _,_  => binint_default
+end.
+
+Function sem_mod (v1:val) (t1:type) (v2: val) (t2:type) : option val :=
+  match classify_binint t1 t2 with
+  | binint_case_ii Unsigned =>
+      match v1, v2 with
+      | Vint n1, Vint n2 =>
+          if Int.eq n2 Int.zero then None else Some (Vint (Int.modu n1 n2))
+      | _, _ => None
+      end
+  | binint_case_ii Signed =>
+      match v1,v2 with
+      | Vint n1, Vint n2 =>
+          if Int.eq n2 Int.zero
+          || Int.eq n1 (Int.repr Int.min_signed) && Int.eq n2 Int.mone
+          then None else Some (Vint (Int.mods n1 n2))
+      | _, _ => None
+      end
+  | binint_default =>
+      None
+  end.
+
+Function sem_and (v1:val) (t1:type) (v2: val) (t2:type) : option val :=
+  match classify_binint t1 t2 with
+  | binint_case_ii sg =>
+      match v1, v2 with
+      | Vint n1, Vint n2 => Some (Vint(Int.and n1 n2))
+      | _, _ => None
+      end
+  | binint_default => None
+  end.
+
+Function sem_or (v1:val) (t1:type) (v2: val) (t2:type) : option val :=
+  match classify_binint t1 t2 with
+  | binint_case_ii sg =>
+      match v1, v2 with
+      | Vint n1, Vint n2 => Some (Vint(Int.or n1 n2))
+      | _, _ => None
+      end
+  | binint_default => None
+  end.
+
+Function sem_xor (v1:val) (t1:type) (v2: val) (t2:type) : option val :=
+  match classify_binint t1 t2 with
+  | binint_case_ii sg =>
+      match v1, v2 with
+      | Vint n1, Vint n2 => Some (Vint(Int.xor n1 n2))
+      | _, _ => None
+      end
+  | binint_default => None
+  end.
+
+(** *** Shifts *)
+
+Inductive classify_shift_cases : Type:=
+  | shift_case_ii(s: signedness) (**r int , int *)
+  | shift_default.
+
+Definition classify_shift (ty1: type) (ty2: type) :=
+  match typeconv ty1, typeconv ty2 with
+  | Tint I32 Unsigned _, Tint _ _ _ => shift_case_ii Unsigned
+  | Tint _ _ _, Tint _ _ _ => shift_case_ii Signed
+  | _,_  => shift_default
+end.
+
+Function sem_shl (v1:val) (t1:type) (v2: val) (t2:type) : option val :=
+  match classify_shift t1 t2 with
+  | shift_case_ii sg =>
+      match v1, v2 with
+      | Vint n1, Vint n2 =>
+         if Int.ltu n2 Int.iwordsize then Some (Vint(Int.shl n1 n2)) else None
+      | _, _ => None
+      end
+  | shift_default => None
+  end.
+
+Function sem_shr (v1: val) (t1: type) (v2: val) (t2: type): option val :=
+  match classify_shift t1 t2 with 
+  | shift_case_ii Unsigned =>
+      match v1,v2 with 
+      | Vint n1, Vint n2 =>
+          if Int.ltu n2 Int.iwordsize then Some (Vint (Int.shru n1 n2)) else None
+      | _,_ => None
+      end
+   | shift_case_ii Signed =>
+      match v1,v2 with
+      | Vint n1,  Vint n2 =>
+          if Int.ltu n2 Int.iwordsize then Some (Vint (Int.shr n1 n2)) else None
+      | _,  _ => None
+      end
+   | shift_default =>
+      None
+   end.
+
+(** *** Comparisons *)
+
+Inductive classify_cmp_cases : Type:=
+  | cmp_case_ii(s: signedness) (**r int, int *)
+  | cmp_case_pp                (**r pointer, pointer *)
+  | cmp_case_ff                (**r float , float *)
+  | cmp_case_if(s: signedness) (**r int, float *)
+  | cmp_case_fi(s: signedness) (**r float, int *)
+  | cmp_default.
+
+Definition classify_cmp (ty1: type) (ty2: type) :=
+  match typeconv ty1, typeconv ty2 with 
+  | Tint I32 Unsigned _ , Tint _ _ _ => cmp_case_ii Unsigned
+  | Tint _ _ _ , Tint I32 Unsigned _ => cmp_case_ii Unsigned
+  | Tint _ _ _ , Tint _ _ _ => cmp_case_ii Signed
+  | Tfloat _ _ , Tfloat _ _ => cmp_case_ff
+  | Tint _ sg _, Tfloat _ _ => cmp_case_if sg
+  | Tfloat _ _, Tint _ sg _ => cmp_case_fi sg
+  | Tpointer _ _ , Tpointer _ _ => cmp_case_pp
+  | Tpointer _ _ , Tint _ _ _ => cmp_case_pp
+  | Tint _ _ _, Tpointer _ _ => cmp_case_pp
+  | _ , _ => cmp_default
+  end.
+
+Function sem_cmp_mismatch (c: comparison): option val :=
+  match c with
+  | Ceq =>  Some Vfalse
+  | Cne =>  Some Vtrue
+  | _   => None
+  end.
+
+Function sem_cmp (c:comparison)
+                  (v1: val) (t1: type) (v2: val) (t2: type)
+                  (m: mem): option val :=
+  match classify_cmp t1 t2 with
+  | cmp_case_ii Signed =>
+      match v1,v2 with
+      | Vint n1, Vint n2 => Some (Val.of_bool (Int.cmp c n1 n2))
+      | _,  _ => None
+      end
+  | cmp_case_ii Unsigned =>
+      match v1,v2 with
+      | Vint n1, Vint n2 => Some (Val.of_bool (Int.cmpu c n1 n2))
+      | _,  _ => None
+      end
+  | cmp_case_pp =>
+      match v1,v2 with
+      | Vint n1, Vint n2 => Some (Val.of_bool (Int.cmpu c n1 n2))
+      | Vptr b1 ofs1,  Vptr b2 ofs2  =>
+          if Mem.valid_pointer m b1 (Int.unsigned ofs1)
+          && Mem.valid_pointer m b2 (Int.unsigned ofs2) then
+            if zeq b1 b2
+            then Some (Val.of_bool (Int.cmpu c ofs1 ofs2))
+            else sem_cmp_mismatch c
+          else None
+      | Vptr b ofs, Vint n =>
+          if Int.eq n Int.zero then sem_cmp_mismatch c else None
+      | Vint n, Vptr b ofs =>
+          if Int.eq n Int.zero then sem_cmp_mismatch c else None
+      | _,  _ => None
+      end
+  | cmp_case_ff =>
+      match v1,v2 with
+      | Vfloat f1, Vfloat f2 => Some (Val.of_bool (Float.cmp c f1 f2))  
+      | _,  _ => None
+      end
+  | cmp_case_if sg =>
+      match v1, v2 with
+      | Vint n1, Vfloat n2 => Some (Val.of_bool (Float.cmp c (cast_int_float sg n1) n2))
+      | _, _ => None
+      end
+  | cmp_case_fi sg =>
+      match v1, v2 with
+      | Vfloat n1, Vint n2 => Some (Val.of_bool (Float.cmp c n1 (cast_int_float sg n2)))
+      | _, _ => None
+      end
+  | cmp_default => None
+  end.
+
+(** ** Function applications *)
+
+Inductive classify_fun_cases : Type:=
+  | fun_case_f (targs: typelist) (tres: type) (**r (pointer to) function *)
+  | fun_default.
+
+Definition classify_fun (ty: type) :=
+  match ty with 
+  | Tfunction args res => fun_case_f args res
+  | Tpointer (Tfunction args res) _ => fun_case_f args res
+  | _ => fun_default
+  end.
+
+(** * Combined semantics of unary and binary operators *)
+
+Definition sem_unary_operation
+            (op: unary_operation) (v: val) (ty: type): option val :=
+  match op with
+  | Onotbool => sem_notbool v ty
+  | Onotint => sem_notint v ty
+  | Oneg => sem_neg v ty
+  end.
+
+Definition sem_binary_operation
+    (op: binary_operation)
+    (v1: val) (t1: type) (v2: val) (t2:type)
+    (m: mem): option val :=
+  match op with
+  | Oadd => sem_add v1 t1 v2 t2
+  | Osub => sem_sub v1 t1 v2 t2 
+  | Omul => sem_mul v1 t1 v2 t2
+  | Omod => sem_mod v1 t1 v2 t2
+  | Odiv => sem_div v1 t1 v2 t2 
+  | Oand => sem_and v1 t1 v2 t2
+  | Oor  => sem_or v1 t1 v2 t2
+  | Oxor  => sem_xor v1 t1 v2 t2
+  | Oshl => sem_shl v1 t1 v2 t2
+  | Oshr  => sem_shr v1 t1 v2 t2   
+  | Oeq => sem_cmp Ceq v1 t1 v2 t2 m
+  | One => sem_cmp Cne v1 t1 v2 t2 m
+  | Olt => sem_cmp Clt v1 t1 v2 t2 m
+  | Ogt => sem_cmp Cgt v1 t1 v2 t2 m
+  | Ole => sem_cmp Cle v1 t1 v2 t2 m
+  | Oge => sem_cmp Cge v1 t1 v2 t2 m
+  end.
+
+Definition sem_incrdecr (id: incr_or_decr) (v: val) (ty: type) :=
+  match id with
+  | Incr => sem_add v ty (Vint Int.one) type_int32s
+  | Decr => sem_sub v ty (Vint Int.one) type_int32s
+  end.
