cfrontend/Ctypes.v
@@ -1,0 +1,546 @@
+(* *********************************************************************)
+(*                                                                     *)
+(*              The Compcert verified compiler                         *)
+(*                                                                     *)
+(*          Xavier Leroy, INRIA Paris-Rocquencourt                     *)
+(*                                                                     *)
+(*  Copyright Institut National de Recherche en Informatique et en     *)
+(*  Automatique.  All rights reserved.  This file is distributed       *)
+(*  under the terms of the GNU General Public License as published by  *)
+(*  the Free Software Foundation, either version 2 of the License, or  *)
+(*  (at your option) any later version.  This file is also distributed *)
+(*  under the terms of the INRIA Non-Commercial License Agreement.     *)
+(*                                                                     *)
+(* *********************************************************************)
+
+(** Type expressions for the Compcert C and Clight languages *)
+
+Require Import Coqlib.
+Require Import AST.
+Require Import Errors.
+
+(** * Syntax of types *)
+
+(** Compcert C types are similar to those of C.  They include numeric types,
+  pointers, arrays, function types, and composite types (struct and 
+  union).  Numeric types (integers and floats) fully specify the
+  bit size of the type.  An integer type is a pair of a signed/unsigned
+  flag and a bit size: 8, 16, or 32 bits, or the special [IBool] size
+  standing for the C99 [_Bool] type. *)
+
+Inductive signedness : Type :=
+  | Signed: signedness
+  | Unsigned: signedness.
+
+Inductive intsize : Type :=
+  | I8: intsize
+  | I16: intsize
+  | I32: intsize
+  | IBool: intsize.
+
+(** Float types come in two sizes: 32 bits (single precision)
+  and 64-bit (double precision). *)
+
+Inductive floatsize : Type :=
+  | F32: floatsize
+  | F64: floatsize.
+
+(** Every type carries a set of attributes.  Currently, only one
+  attribute is modeled: [volatile]. *)
+
+Record attr : Type := mk_attr {
+  attr_volatile: bool
+}.
+
+Definition noattr := {| attr_volatile := false |}.
+
+(** The syntax of type expressions.  Some points to note:
+- Array types [Tarray n] carry the size [n] of the array.
+  Arrays with unknown sizes are represented by pointer types.
+- Function types [Tfunction targs tres] specify the number and types
+  of the function arguments (list [targs]), and the type of the
+  function result ([tres]).  Variadic functions and old-style unprototyped
+  functions are not supported.
+- In C, struct and union types are named and compared by name.
+  This enables the definition of recursive struct types such as
+<<
+  struct s1 { int n; struct * s1 next; };
+>>
+  Note that recursion within types must go through a pointer type.
+  For instance, the following is not allowed in C.
+<<
+  struct s2 { int n; struct s2 next; };
+>>
+  In Compcert C, struct and union types [Tstruct id fields] and
+  [Tunion id fields] are compared by structure: the [fields]
+  argument gives the names and types of the members.  The identifier
+  [id] is a local name which can be used in conjuction with the
+  [Tcomp_ptr] constructor to express recursive types.  [Tcomp_ptr id]
+  stands for a pointer type to the nearest enclosing [Tstruct]
+  or [Tunion] type named [id].  For instance. the structure [s1]
+  defined above in C is expressed by
+<<
+  Tstruct "s1" (Fcons "n" (Tint I32 Signed)
+               (Fcons "next" (Tcomp_ptr "s1")
+               Fnil))
+>>
+  Note that the incorrect structure [s2] above cannot be expressed at
+  all, since [Tcomp_ptr] lets us refer to a pointer to an enclosing
+  structure or union, but not to the structure or union directly.
+*)
+
+Inductive type : Type :=
+  | Tvoid: type                                    (**r the [void] type *)
+  | Tint: intsize -> signedness -> attr -> type    (**r integer types *)
+  | Tfloat: floatsize -> attr -> type              (**r floating-point types *)
+  | Tpointer: type -> attr -> type                 (**r pointer types ([*ty]) *)
+  | Tarray: type -> Z -> attr -> type              (**r array types ([ty[len]]) *)
+  | Tfunction: typelist -> type -> type            (**r function types *)
+  | Tstruct: ident -> fieldlist -> attr -> type    (**r struct types *)
+  | Tunion: ident -> fieldlist -> attr -> type     (**r union types *)
+  | Tcomp_ptr: ident -> attr -> type               (**r pointer to named struct or union *)
+
+with typelist : Type :=
+  | Tnil: typelist
+  | Tcons: type -> typelist -> typelist
+
+with fieldlist : Type :=
+  | Fnil: fieldlist
+  | Fcons: ident -> type -> fieldlist -> fieldlist.
+
+Lemma type_eq: forall (ty1 ty2: type), {ty1=ty2} + {ty1<>ty2}
+with typelist_eq: forall (tyl1 tyl2: typelist), {tyl1=tyl2} + {tyl1<>tyl2}
+with fieldlist_eq: forall (fld1 fld2: fieldlist), {fld1=fld2} + {fld1<>fld2}.
+Proof.
+  assert (forall (x y: intsize), {x=y} + {x<>y}). decide equality.
+  assert (forall (x y: signedness), {x=y} + {x<>y}). decide equality.
+  assert (forall (x y: floatsize), {x=y} + {x<>y}). decide equality.
+  assert (forall (x y: attr), {x=y} + {x<>y}). decide equality. apply bool_dec.
+  generalize ident_eq zeq. intros E1 E2. 
+  decide equality.
+  decide equality.
+  generalize ident_eq. intros E1.
+  decide equality.
+Defined.
+
+Opaque type_eq typelist_eq fieldlist_eq.
+
+(** Extract the attributes of a type. *)
+
+Definition attr_of_type (ty: type) :=
+  match ty with
+  | Tvoid => noattr
+  | Tint sz si a => a
+  | Tfloat sz a => a
+  | Tpointer elt a => a
+  | Tarray elt sz a => a
+  | Tfunction args res => noattr
+  | Tstruct id fld a => a
+  | Tunion id fld a => a
+  | Tcomp_ptr id a => a
+  end.
+
+Definition type_int32s := Tint I32 Signed noattr.
+Definition type_bool := Tint IBool Signed noattr.
+
+(** The usual unary conversion.  Promotes small integer types to [signed int32]
+  and degrades array types and function types to pointer types. *)
+
+Definition typeconv (ty: type) : type :=
+  match ty with
+  | Tint I32 Unsigned _ => ty
+  | Tint _ _ a          => Tint I32 Signed a
+  | Tarray t sz a       => Tpointer t a
+  | Tfunction _ _       => Tpointer ty noattr
+  | _                   => ty
+  end.
+
+(** * Operations over types *)
+
+(** Natural alignment of a type, in bytes. *)
+
+Fixpoint alignof (t: type) : Z :=
+  match t with
+  | Tvoid => 1
+  | Tint I8 _ _ => 1
+  | Tint I16 _ _ => 2
+  | Tint I32 _ _ => 4
+  | Tint IBool _ _ => 1
+  | Tfloat F32 _ => 4
+  | Tfloat F64 _ => 8
+  | Tpointer _ _ => 4
+  | Tarray t' _ _ => alignof t'
+  | Tfunction _ _ => 1
+  | Tstruct _ fld _ => alignof_fields fld
+  | Tunion _ fld _ => alignof_fields fld
+  | Tcomp_ptr _ _ => 4
+  end
+
+with alignof_fields (f: fieldlist) : Z :=
+  match f with
+  | Fnil => 1
+  | Fcons id t f' => Zmax (alignof t) (alignof_fields f')
+  end.
+
+Scheme type_ind2 := Induction for type Sort Prop
+  with fieldlist_ind2 := Induction for fieldlist Sort Prop.
+
+Lemma alignof_1248:
+  forall t, alignof t = 1 \/ alignof t = 2 \/ alignof t = 4 \/ alignof t = 8
+with alignof_fields_1248:
+  forall f, alignof_fields f = 1 \/ alignof_fields f = 2 \/ alignof_fields f = 4 \/ alignof_fields f = 8.
+Proof.
+  induction t; simpl; auto.
+  destruct i; auto.
+  destruct f; auto.
+  induction f; simpl; auto.
+  rewrite Zmax_spec. destruct (zlt (alignof_fields f) (alignof t)); auto.
+Qed.
+
+Lemma alignof_pos:
+  forall t, alignof t > 0.
+Proof.
+  intros. generalize (alignof_1248 t). omega.
+Qed.
+
+Lemma alignof_fields_pos:
+  forall f, alignof_fields f > 0.
+Proof.
+  intros. generalize (alignof_fields_1248 f). omega.
+Qed.
+
+(** Size of a type, in bytes. *)
+
+Fixpoint sizeof (t: type) : Z :=
+  match t with
+  | Tvoid => 1
+  | Tint I8 _ _ => 1
+  | Tint I16 _ _ => 2
+  | Tint I32 _ _ => 4
+  | Tint IBool _ _ => 1
+  | Tfloat F32 _ => 4
+  | Tfloat F64 _ => 8
+  | Tpointer _ _ => 4
+  | Tarray t' n _ => sizeof t' * Zmax 1 n
+  | Tfunction _ _ => 1
+  | Tstruct _ fld _ => align (Zmax 1 (sizeof_struct fld 0)) (alignof t)
+  | Tunion _ fld _ => align (Zmax 1 (sizeof_union fld)) (alignof t)
+  | Tcomp_ptr _ _ => 4
+  end
+
+with sizeof_struct (fld: fieldlist) (pos: Z) {struct fld} : Z :=
+  match fld with
+  | Fnil => pos
+  | Fcons id t fld' => sizeof_struct fld' (align pos (alignof t) + sizeof t)
+  end
+
+with sizeof_union (fld: fieldlist) : Z :=
+  match fld with
+  | Fnil => 0
+  | Fcons id t fld' => Zmax (sizeof t) (sizeof_union fld')
+  end.
+
+Lemma sizeof_pos:
+  forall t, sizeof t > 0.
+Proof.
+  intro t0.
+  apply (type_ind2 (fun t => sizeof t > 0)
+                   (fun f => sizeof_union f >= 0 /\ forall pos, pos >= 0 -> sizeof_struct f pos >= 0));
+  intros; simpl; auto; try omega.
+  destruct i; omega.
+  destruct f; omega.
+  apply Zmult_gt_0_compat. auto. generalize (Zmax1 1 z); omega.
+  destruct H. 
+  generalize (align_le (Zmax 1 (sizeof_struct f 0)) (alignof_fields f) (alignof_fields_pos f)). 
+  generalize (Zmax1 1 (sizeof_struct f 0)). omega. 
+  generalize (align_le (Zmax 1 (sizeof_union f)) (alignof_fields f) (alignof_fields_pos f)). 
+  generalize (Zmax1 1 (sizeof_union f)). omega. 
+  split. omega. auto.
+  destruct H0. split; intros.
+  generalize (Zmax2 (sizeof t) (sizeof_union f)). omega.
+  apply H1. 
+  generalize (align_le pos (alignof t) (alignof_pos t)). omega.
+Qed.
+
+Lemma sizeof_struct_incr:
+  forall fld pos, pos <= sizeof_struct fld pos.
+Proof.
+  induction fld; intros; simpl. omega. 
+  eapply Zle_trans. 2: apply IHfld.
+  apply Zle_trans with (align pos (alignof t)). 
+  apply align_le. apply alignof_pos. 
+  assert (sizeof t > 0) by apply sizeof_pos. omega.
+Qed.
+
+Lemma sizeof_alignof_compat:
+  forall t, (alignof t | sizeof t).
+Proof.
+  induction t; simpl; try (apply Zdivide_refl).
+  apply Zdivide_mult_l. auto.
+  apply align_divides. apply alignof_fields_pos.
+  apply align_divides. apply alignof_fields_pos.
+Qed.
+
+(** Byte offset for a field in a struct or union.
+  Field are laid out consecutively, and padding is inserted
+  to align each field to the natural alignment for its type. *)
+
+Open Local Scope string_scope.
+
+Fixpoint field_offset_rec (id: ident) (fld: fieldlist) (pos: Z)
+                              {struct fld} : res Z :=
+  match fld with
+  | Fnil => Error (MSG "Unknown field " :: CTX id :: nil)
+  | Fcons id' t fld' =>
+      if ident_eq id id'
+      then OK (align pos (alignof t))
+      else field_offset_rec id fld' (align pos (alignof t) + sizeof t)
+  end.
+
+Definition field_offset (id: ident) (fld: fieldlist) : res Z :=
+  field_offset_rec id fld 0.
+
+Fixpoint field_type (id: ident) (fld: fieldlist) {struct fld} : res type :=
+  match fld with
+  | Fnil => Error (MSG "Unknown field " :: CTX id :: nil)
+  | Fcons id' t fld' => if ident_eq id id' then OK t else field_type id fld'
+  end.
+
+(** Some sanity checks about field offsets.  First, field offsets are 
+  within the range of acceptable offsets. *)
+
+Remark field_offset_rec_in_range:
+  forall id ofs ty fld pos,
+  field_offset_rec id fld pos = OK ofs -> field_type id fld = OK ty ->
+  pos <= ofs /\ ofs + sizeof ty <= sizeof_struct fld pos.
+Proof.
+  intros until ty. induction fld; simpl.
+  congruence.
+  destruct (ident_eq id i); intros.
+  inv H. inv H0. split. apply align_le. apply alignof_pos. apply sizeof_struct_incr.
+  exploit IHfld; eauto. intros [A B]. split; auto. 
+  eapply Zle_trans; eauto. apply Zle_trans with (align pos (alignof t)).
+  apply align_le. apply alignof_pos. generalize (sizeof_pos t). omega. 
+Qed.
+
+Lemma field_offset_in_range:
+  forall sid fld a fid ofs ty,
+  field_offset fid fld = OK ofs -> field_type fid fld = OK ty ->
+  0 <= ofs /\ ofs + sizeof ty <= sizeof (Tstruct sid fld a).
+Proof.
+  intros. exploit field_offset_rec_in_range; eauto. intros [A B].
+  split. auto.  simpl. eapply Zle_trans. eauto.
+  eapply Zle_trans. eapply Zle_max_r. apply align_le. apply alignof_fields_pos.
+Qed.
+
+(** Second, two distinct fields do not overlap *)
+
+Lemma field_offset_no_overlap:
+  forall id1 ofs1 ty1 id2 ofs2 ty2 fld,
+  field_offset id1 fld = OK ofs1 -> field_type id1 fld = OK ty1 ->
+  field_offset id2 fld = OK ofs2 -> field_type id2 fld = OK ty2 ->
+  id1 <> id2 ->
+  ofs1 + sizeof ty1 <= ofs2 \/ ofs2 + sizeof ty2 <= ofs1.
+Proof.
+  intros until ty2. intros fld0 A B C D NEQ.
+  assert (forall fld pos,
+  field_offset_rec id1 fld pos = OK ofs1 -> field_type id1 fld = OK ty1 ->
+  field_offset_rec id2 fld pos = OK ofs2 -> field_type id2 fld = OK ty2 ->
+  ofs1 + sizeof ty1 <= ofs2 \/ ofs2 + sizeof ty2 <= ofs1).
+  induction fld; intro pos; simpl. congruence.
+  destruct (ident_eq id1 i); destruct (ident_eq id2 i).
+  congruence. 
+  subst i. intros. inv H; inv H0.
+  exploit field_offset_rec_in_range. eexact H1. eauto. tauto.  
+  subst i. intros. inv H1; inv H2.
+  exploit field_offset_rec_in_range. eexact H. eauto. tauto. 
+  intros. eapply IHfld; eauto.
+
+  apply H with fld0 0; auto.
+Qed.
+
+(** Third, if a struct is a prefix of another, the offsets of common fields
+    are the same. *)
+
+Fixpoint fieldlist_app (fld1 fld2: fieldlist) {struct fld1} : fieldlist :=
+  match fld1 with
+  | Fnil => fld2
+  | Fcons id ty fld => Fcons id ty (fieldlist_app fld fld2)
+  end.
+
+Lemma field_offset_prefix:
+  forall id ofs fld2 fld1,
+  field_offset id fld1 = OK ofs ->
+  field_offset id (fieldlist_app fld1 fld2) = OK ofs.
+Proof.
+  intros until fld2.
+  assert (forall fld1 pos, 
+    field_offset_rec id fld1 pos = OK ofs ->
+    field_offset_rec id (fieldlist_app fld1 fld2) pos = OK ofs).
+  induction fld1; intros pos; simpl. congruence.
+  destruct (ident_eq id i); auto.
+  intros. unfold field_offset; auto. 
+Qed.
+
+(** Fourth, the position of each field respects its alignment. *)
+
+Lemma field_offset_aligned:
+  forall id fld ofs ty,
+  field_offset id fld = OK ofs -> field_type id fld = OK ty ->
+  (alignof ty | ofs).
+Proof.
+  assert (forall id ofs ty fld pos,
+          field_offset_rec id fld pos = OK ofs -> field_type id fld = OK ty ->
+          (alignof ty | ofs)).
+  induction fld; simpl; intros.
+  discriminate.
+  destruct (ident_eq id i). inv H; inv H0. 
+  apply align_divides. apply alignof_pos. 
+  eapply IHfld; eauto.
+  intros. eapply H with (pos := 0); eauto.
+Qed.
+
+(** The [access_mode] function describes how a l-value of the given
+type must be accessed:
+- [By_value ch]: access by value, i.e. by loading from the address
+  of the l-value using the memory chunk [ch];
+- [By_reference]: access by reference, i.e. by just returning
+  the address of the l-value (used for arrays and functions);
+- [By_copy]: access is by reference, assignment is by copy
+  (used for [struct] and [union] types)
+- [By_nothing]: no access is possible, e.g. for the [void] type.
+*)
+
+Inductive mode: Type :=
+  | By_value: memory_chunk -> mode
+  | By_reference: mode
+  | By_copy: mode
+  | By_nothing: mode.
+
+Definition access_mode (ty: type) : mode :=
+  match ty with
+  | Tint I8 Signed _ => By_value Mint8signed
+  | Tint I8 Unsigned _ => By_value Mint8unsigned
+  | Tint I16 Signed _ => By_value Mint16signed
+  | Tint I16 Unsigned _ => By_value Mint16unsigned
+  | Tint I32 _ _ => By_value Mint32
+  | Tint IBool _ _ => By_value Mint8unsigned
+  | Tfloat F32 _ => By_value Mfloat32
+  | Tfloat F64 _ => By_value Mfloat64
+  | Tvoid => By_nothing
+  | Tpointer _ _ => By_value Mint32
+  | Tarray _ _ _ => By_reference
+  | Tfunction _ _ => By_reference
+  | Tstruct _ _ _ => By_copy
+  | Tunion _ _ _ => By_copy
+  | Tcomp_ptr _ _ => By_nothing
+end.
+
+(** For the purposes of the semantics and the compiler, a type denotes
+  a volatile access if it carries the [volatile] attribute and it is
+  accessed by value. *)
+
+Definition type_is_volatile (ty: type) : bool :=
+  match access_mode ty with
+  | By_value _ => attr_volatile (attr_of_type ty)
+  | _          => false
+  end.
+
+(** Unroll the type of a structure or union field, substituting
+    [Tcomp_ptr] by a pointer to the structure. *)
+
+Section UNROLL_COMPOSITE.
+
+Variable cid: ident.
+Variable comp: type.
+
+Fixpoint unroll_composite (ty: type) : type :=
+  match ty with
+  | Tvoid => ty
+  | Tint _ _ _ => ty
+  | Tfloat _ _ => ty
+  | Tpointer t1 a => Tpointer (unroll_composite t1) a
+  | Tarray t1 sz a => Tarray (unroll_composite t1) sz a
+  | Tfunction t1 t2 => Tfunction (unroll_composite_list t1) (unroll_composite t2)
+  | Tstruct id fld a => if ident_eq id cid then ty else Tstruct id (unroll_composite_fields fld) a
+  | Tunion id fld a => if ident_eq id cid then ty else Tunion id (unroll_composite_fields fld) a
+  | Tcomp_ptr id a => if ident_eq id cid then Tpointer comp a else ty
+  end
+
+with unroll_composite_list (tl: typelist) : typelist :=
+  match tl with
+  | Tnil => Tnil
+  | Tcons t1 tl' => Tcons (unroll_composite t1) (unroll_composite_list tl')
+  end
+
+with unroll_composite_fields (fld: fieldlist) : fieldlist :=
+  match fld with
+  | Fnil => Fnil
+  | Fcons id ty fld' => Fcons id (unroll_composite ty) (unroll_composite_fields fld')
+  end.
+
+Lemma alignof_unroll_composite:
+  forall ty, alignof (unroll_composite ty) = alignof ty.
+Proof.
+  apply (type_ind2 (fun ty => alignof (unroll_composite ty) = alignof ty)
+                   (fun fld => alignof_fields (unroll_composite_fields fld) = alignof_fields fld));
+  simpl; intros; auto.
+  destruct (ident_eq i cid); auto. 
+  destruct (ident_eq i cid); auto. 
+  destruct (ident_eq i cid); auto.
+  decEq; auto.
+Qed.
+
+Lemma sizeof_unroll_composite:
+  forall ty, sizeof (unroll_composite ty) = sizeof ty.
+Proof.
+Opaque alignof.
+  apply (type_ind2 (fun ty => sizeof (unroll_composite ty) = sizeof ty)
+                   (fun fld => 
+                      sizeof_union (unroll_composite_fields fld) = sizeof_union fld
+                   /\ forall pos,
+                      sizeof_struct (unroll_composite_fields fld) pos = sizeof_struct fld pos));
+  simpl; intros; auto.
+  congruence.
+  destruct H. rewrite <- (alignof_unroll_composite (Tstruct i f a)).
+  simpl. destruct (ident_eq i cid); simpl. auto. rewrite H0; auto.
+  destruct H. rewrite <- (alignof_unroll_composite (Tunion i f a)).
+  simpl. destruct (ident_eq i cid); simpl. auto. rewrite H; auto.
+  destruct (ident_eq i cid); auto.
+  destruct H0. split. congruence.
+  intros. rewrite alignof_unroll_composite. rewrite H1. rewrite H. auto.
+Qed.
+
+End UNROLL_COMPOSITE.
+
+(** Extracting a type list from a function parameter declaration. *)
+
+Fixpoint type_of_params (params: list (ident * type)) : typelist :=
+  match params with
+  | nil => Tnil
+  | (id, ty) :: rem => Tcons ty (type_of_params rem)
+  end.
+
+(** Translating C types to Cminor types and function signatures. *)
+
+Definition typ_of_type (t: type) : AST.typ :=
+  match t with
+  | Tfloat _ _ => AST.Tfloat
+  | _ => AST.Tint
+  end.
+
+Definition opttyp_of_type (t: type) : option AST.typ :=
+  match t with
+  | Tvoid => None
+  | Tfloat _ _ => Some AST.Tfloat
+  | _ => Some AST.Tint
+  end.
+
+Fixpoint typlist_of_typelist (tl: typelist) : list AST.typ :=
+  match tl with
+  | Tnil => nil
+  | Tcons hd tl => typ_of_type hd :: typlist_of_typelist tl
+  end.
+
+Definition signature_of_type (args: typelist) (res: type) : signature :=
+  mksignature (typlist_of_typelist args) (opttyp_of_type res).
